day3.thy
@@ -54,11 +54,13 @@ definition example_input::string where "example_input = ''
 .#..#...#.#
 ''"
 
-value "part1 example_input"
+lemma "part1 example_input = 7"
+  by eval
 
 text "For part 2 the example should return 336"
 
-value "part2 example_input"
+lemma "part2 example_input = 336"
+  by eval
 
 export_code "part1" "part2" in Haskell module_name Solution
 
